SP1Clean.lean
@@ -4,7 +4,6 @@ import SP1Clean.Proofs.Chips.AddChip.Formal
 import SP1Clean.Native.Chips.AddiChip.Defs
 import SP1Clean.Proofs.Chips.AddiChip.Formal
 import SP1Clean.Proofs.Chips.AddiChip.Bridge
-import SP1Clean.Proofs.Chips.AddiChip.Advance
 import SP1Clean.Proofs.Chips.AddwChip.Bridge
 import SP1Clean.Native.Chips.AddwChip.Defs
 import SP1Clean.Proofs.Chips.AddwChip.Formal
@@ -109,7 +108,6 @@ import SP1Clean.Proofs.Chips.StoreWordChip.Bridge
 import SP1Clean.Native.Chips.StoreWordChip.Defs
 import SP1Clean.Proofs.Chips.StoreWordChip.Formal
 import SP1Clean.Proofs.Chips.SubChip.Bridge
-import SP1Clean.Proofs.Chips.SubChip.Advance
 import SP1Clean.Native.Chips.SubChip.Defs
 import SP1Clean.Proofs.Chips.SubChip.Formal
 import SP1Clean.Proofs.Chips.SubwChip.Bridge
